\documentclass{article}

\usepackage{amsmath, amsfonts, amssymb, amsthm}
\usepackage{cancel}
\usepackage{tcolorbox}

\begin{document}

\title{Infinite summation for perimeter of an ellipse}
\author{dnzc}
\date{}

\maketitle

\tableofcontents
\newpage



\section{Introduction}
Using an arc length integral it is possible to show that the circumference, $C$, of an ellipse with height 2b and width 2a is
\[C = 4a\int_{0}^{\pi/2}\sqrt{1 + (\frac{a^2}{b^2}-1)\sin^2x}\,\,dx\]
This is derived in the appendix. 
In section 1.1 we setup the integral to be turned into an infinite sigma summation. 
In later sections I go through each case established in 1.1 to derive two infinite sums equal to the circumference, then equate them.
\subsection{Problem setup}
Let $c = \frac{a^2}{b^2}-1$. Then the integral will be
\[C = 4a\int_{0}^{\pi/2}(1 + c\sin^2x)^\frac{1}{2}\,\,dx\]
We will use the binomial expansion for nonintegers on $(1 + c\sin^2x)^\frac{1}{2}$, then integrate term by term.\\
In the next sections we consider the 2 cases of c: $|c| \leq 1$, and $|c| \geq 1$.



\section{Case 1}
We solve the case of $|c| \geq 1$.
\begin{equation}
\begin{split}
	C = 4a\int_{0}^{\pi/2}(1 + c\sin^2x)^\frac{1}{2}\,\,dx\\
	= 4a\sqrt{c+1}\int_{0}^{\pi/2}(1 - \frac{c}{c+1}\cos^2x)^\frac{1}{2}\,\,dx
\end{split}
\end{equation}
Note that $\because c=\frac{a^2}{b^2} - 1 > -1, |c|\geq 1 \implies c\geq 1$\\
$\therefore |\frac{c}{c+1}cos^2x|<1\forall x \in \mathbb{R}$\\
So now we can use the binomial expansion.
\begin{equation*}
\begin{split}
	\left(1 - \frac{c}{c+1}\cos^2x\right)^\frac{1}{2}
	= 1 + \sum_{k\geq 1} \frac{\frac{1}{2}\times-\frac{1}{2}\dots\times(\frac{1}{2}-k+1)}{k!}\left(-\frac{c}{c+1}\cos^2x\right)^k\\
	= 1 + \sum_{k\geq 1} \frac{\prod_{n=1}^{k}(2n-3)}{2^kk!}\left(\frac{c}{c+1}\right)^k\cos^{2k}x
\end{split}
\end{equation*}
Substitute this back into (1):
\begin{equation*}
\begin{split}
	C = 4a\sqrt{c+1}\int_{0}^{\pi/2}\left(
	1 + \sum_{k\geq 1} \frac{\prod_{n=1}^{k}(2n-3)}{2^kk!}\left(\frac{c}{c+1}\right)^k\cos^{2k}x
	\right)dx\\
	= 2\pi a\sqrt{c+1} + 4a\sqrt{c+1}\int_{0}^{\pi/2}\sum_{k\geq 1} \frac{\prod_{n=1}^{k}(2n-3)}{2^kk!}\left(\frac{c}{c+1}\right)^k\cos^{2k}x\,dx\\
\end{split}
\end{equation*}
Integrating term by term (sum and integral are interchanged):
\begin{equation}
\begin{split}
	= 2\pi a\sqrt{c+1} +
	4a\sqrt{c+1}\sum_{k\geq 1}\left( \frac{\prod_{n=1}^{k}(2n-3)}{2^kk!}\left(\frac{c}{c+1}\right)^k\int_{0}^{\pi/2}\cos^{2k}x\,dx\right)\\
\end{split}
\end{equation}

It is proved in the appendix that $\int_{0}^{\pi/2}\cos^{2k}(x)\,\,dx = \frac{\pi}{2}\prod_{n=1}^{k}\frac{2n-1}{2n}$


Substitute this back into (2):
\begin{equation}
\begin{split}
	C = 
	2\pi a\sqrt{c+1} +
	4a\sqrt{c+1}\sum_{k\geq 1}\left( \frac{\prod_{n=1}^{k}(2n-3)}{2^kk!}\left(\frac{c}{c+1}\right)^k\frac{\pi}{2}\prod_{n=1}^{k}\frac{2n-1}{2n}\right)\\
	= 2\pi a\sqrt{c+1} +
	2\pi a\sqrt{c+1}\sum_{k\geq 1}\left( \frac{\prod_{n=1}^{k}(2n-3)\prod_{n=1}^{k}(2n-1)}{2^kk!\prod_{n=1}^k(2n)}\left(\frac{c}{c+1}\right)^k\right)\\
	= 2\pi a\sqrt{c+1} \left(1 + 
	\sum_{k\geq 1}\left( \frac{\prod_{n=1}^{k}(2n-3)(2n-1)}{4^k(k!)^2}\left(\frac{c}{c+1}\right)^k\right)\right)\\
\end{split}
\end{equation}

Note
\begin{equation}
\begin{split}
	\prod_{n=1}^k(2n-3)(2n-1)
	= (-1 \times 1) \times (1\times 3)\times\dots\times[(2k-3)\times(2k-1)]\\
	= -1 \times 1^2 \times 3^2 \times\dots\times(2k-3)^2 \times (2k-1)\\
	= (1-2k)\left[1\times3\times\dots\times(2k-3)\right]^2\\
	= (1-2k)\left[\frac{1\times2\times3\times\dots\times(2k-3)\times(2k-2)}{2\times4\times\dots\times(2k-2)}\right]^2\\
	= \frac{1-2k}{4^{k-1}}\left[\frac{(2k-2)!}{(k-1)!}\right]^2
\end{split}
\end{equation}

Substitute back into (3):
\begin{equation*}
\begin{split}
	C
	= 2\pi a\sqrt{c+1} \left(1 + 
	\sum_{k\geq 1}\left( \frac{(1-2k)\left[\frac{(2k-2)!}{(k-1)!}\right]^2}{4^{k-1}4^k(k!)^2}\left(\frac{c}{c+1}\right)^k\right)\right)\\
	= 2\pi a\sqrt{c+1} \left(1 + 
	\sum_{k\geq 1}\left( \frac{-1}{4^{2k-1}(2k-1)}\left[\frac{(2k-1)(2k-2)!}{k!(k-1)!}\right]^2\left(\frac{c}{c+1}\right)^k\right)\right)\\
	= 2\pi a\sqrt{c+1} \left(1 -
	\sum_{k\geq 1} \frac{4^{1-2k}}{2k-1}{{2k-1}\choose{k-1}}^2\left(\frac{c}{c+1}\right)^k\right)\\
\end{split}
\end{equation*}

Reindex:
\begin{equation*}
\begin{split}
	= 2\pi a\sqrt{c+1} \left(1 -
	\sum_{k\geq 0} \frac{4^{-1-2k}}{2k+1}{{2k+1}\choose k}^2\left(\frac{c}{c+1}\right)^{k+1}\right)\\
\end{split}
\end{equation*}

\begin{tcolorbox}
\begin{equation*}
\begin{split}
	C = \frac{\pi a\sqrt{c+1}}{2} \left(4 -
	\sum_{k=0}^{\infty} \frac{16^{-k}{{2k+1}\choose k}^2}{2k+1}\left(\frac{c}{c+1}\right)^{k+1}\right)\\
\end{split}
\end{equation*}
\end{tcolorbox}



\section{Case 2}
Now we solve the case $|c| \leq 1$.
\begin{equation*}
\begin{split}
	C = 4a\int_{0}^{\pi/2}(1 + c\sin^2x)^\frac{1}{2}\,\,dx
\end{split}
\end{equation*}
Note that $|csin^2x|<1\forall x, 0\leq x < \frac{\pi}{2}$\\
So we can use the binomial expansion.
\begin{equation*}
\begin{split}
	= 4a\int_{0}^{\pi/2}\left(1 + \sum_{k\geq 1}\frac{\frac{1}{2}\times-\frac{1}{2}\times\cdots\times(\frac{1}{2}-k+1)}{k!}(c\sin^2x)^k\right)\,\,dx
\end{split}
\end{equation*}
Integrate term by term:
\begin{equation}
\begin{split}
	= 2\pi a + 4a\sum_{k\geq 1}\frac{\frac{1}{2}\times\cdots\times(\frac{3}{2}-k)}{k!}c^k\int_{0}^{\pi/2}\sin^{2k}x\,\,dx\\
\end{split}
\end{equation}

It is proved in the appendix that 
$\int_{0}^{\pi/2}\sin^{2k}x\,\,dx = \frac{\pi}{2}\prod_{n=1}^k\frac{2n-1}{2n}$\\
Substitute back into (5):
\begin{equation*}
\begin{split}
	C
	= 2\pi a+4a\sum_{k\geq 1}\frac{\frac{1}{2}\times\cdots\times(\frac{3}{2}-k)}{k!}c^k\frac{\pi}{2}\prod_{n=1}^k\frac{2n-1}{2n}\\
	= 2\pi a + 2\pi a\sum_{k\geq 1}\frac{\prod_{n=1}^k(3-2n)\prod_{n=1}^k(2n-1)}{2^kk!\prod_{n=1}^k(2n)}c^k\\
	= 2\pi a\left(1+\sum_{k\geq 1}\frac{\prod_{n=1}^k(2n-3)(2n-1)}{4^k(k!)^2}(-c)^k\right)\\
\end{split}
\end{equation*}
Substitute (4) in:
\begin{equation*}
\begin{split}
	= 2\pi a\left(1+\sum_{k\geq 1}\frac{(1-2k)\left[\frac{(2k-2)!}{(k-1)!}\right]^2}{4^{k-1}4^k(k!)^2}(-c)^k\right)\\
	= 2\pi a\left(1+\sum_{k\geq 1}\frac{-1}{4^{2k-1}(2k-1)}\left[\frac{(2k-1)(2k-2)!}{k!(k-1)!}\right]^2(-c)^k\right)\\
	= 2\pi a\left(1-\sum_{k\geq 1}\frac{4^{1-2k}}{2k-1}{{2k-1}\choose {k-1}}^2(-c)^k\right)\\
\end{split}
\end{equation*}
Reindex:
\begin{equation*}
\begin{split}
	= 2\pi a\left(1-\sum_{k\geq 0}\frac{4^{-1-2k}}{2k+1}{{2k+1}\choose k}^2(-c)^{k+1}\right)\\
\end{split}
\end{equation*}
\begin{tcolorbox}
\begin{equation*}
\begin{split}
	C = \frac{\pi a}{2}\left(4-\sum_{k=0}^{\infty}\frac{16^{-k}{{2k+1}\choose k}^2}{2k+1}(-c)^{k+1}\right)\\
\end{split}
\end{equation*}
\end{tcolorbox}
Note when c=0 (a=b so the ellipse is a circle) the whole summation vanishes so $C$ becomes $2\pi a$.



\section{Summary}
I have derived 2 infinite sums for the circumference, $C$, of an ellipse depending on $|c|$ Where 2a is the width, 2b is the height and $c=\frac{a^2}{b^2}-1$.
\begin{equation*}
\end{equation*}

If $|c| \geq 1$:
\begin{equation*}
\begin{split}
	C = \frac{\pi a\sqrt{c+1}}{2} \left(4 -
	\sum_{k=0}^{\infty} \frac{16^{-k}{{2k+1}\choose k}^2}{2k+1}\left(\frac{c}{c+1}\right)^{k+1}\right)\\
\end{split}
\end{equation*}

If $|c| \leq 1$:
\begin{equation*}
\begin{split}
	C = \frac{\pi a}{2}\left(4-\sum_{k=0}^{\infty}\frac{16^{-k}{{2k+1}\choose k}^2}{2k+1}(-c)^{k+1}\right)\\
\end{split}
\end{equation*}

\subsection{Discovery}
I realized if you plug c=1 into both sums, they must be equal, therefore:
\begin{equation*}
\begin{split}
	\frac{\pi a\sqrt{2}}{2} \left(4 -
	\sum_{k=0}^{\infty} \frac{16^{-k}{{2k+1}\choose k}^2}{2k+1}\left(\frac{1}{2}\right)^{k+1}\right)
	= \frac{\pi a}{2}\left(4-\sum_{k=0}^{\infty}\frac{16^{-k}{{2k+1}\choose k}^2}{2k+1}(-1)^{k+1}\right)\\
\end{split}
\end{equation*}
Now simplify:

\begin{equation*}
\begin{split}
	4\sqrt2 -
	\sqrt2\sum_{k=0}^{\infty} \frac{16^{-k}{{2k+1}\choose k}^2}{2k+1}\left(\frac{1}{2}\right)^{k+1}
	= 4-\sum_{k=0}^{\infty}\frac{16^{-k}{{2k+1}\choose k}^2}{2k+1}(-1)^{k+1}\\
	\sqrt2\sum_{k=0}^{\infty} \frac{16^{-k}{{2k+1}\choose k}^2}{2k+1}\left(\frac{1}{2}\right)^{k+1}
	-\sum_{k=0}^{\infty}\frac{16^{-k}{{2k+1}\choose k}^2}{2k+1}(-1)^{k+1}
	= 4\sqrt2 - 4\\
	\sum_{k=0}^{\infty} \left( \frac{16^{-k}{{2k+1}\choose k}^2\sqrt2}{(2k+1)2^{k+1}}
	- \frac{16^{-k}{{2k+1}\choose k}^2}{2k+1}(-1)^{k+1} \right)
	= 4\sqrt2 - 4\\
	\sum_{k=0}^{\infty} \frac{16^{-k}{{2k+1}\choose k}^2}{(2k+1)} \left( \frac{\sqrt2}{2^{k+1}} - (-1)^{k+1} \right)
	= 4\sqrt2 - 4\\
	\sum_{k=0}^{\infty} \frac{16^{-k}2^{-k}{{2k+1}\choose k}^2}{(2k+1)} \left( \frac{\sqrt2}{2} + (-2)^k \right)
	= 4\sqrt2 - 4\\
\end{split}
\end{equation*}

\begin{tcolorbox}
\begin{equation*}
\begin{split}
	\sum_{k=0}^{\infty} \frac{{{2k+1}\choose k}^2\left( 1 + \sqrt2(-2)^k \right)}{32^k(2k+1)} 
	= 8 - 4\sqrt2\\
\end{split}
\end{equation*}
\end{tcolorbox}
Nice.



\section{Appendix}
% TBA



\end{document}













% temp store of stuff to add to appendix:


We now focus on $\int_{0}^{\pi/2}\cos^{2k}x\,\,dx$, let this be $I_k$.
\begin{equation*}
\begin{split}
	I_k = \int_{0}^{\pi/2}\cos^{2k-1}(x)\cos x\,\,dx\\
	\text{Using IBP:}\\
	= \cancelto{0}{\sin x\cos^{2k-1}x\Big|_{0}^{\pi/2}} - \int_{0}^{\pi/2}(2k-1)\times-\sin^2x\cos^{2k-2}x\,\,dx\\
	= (2k-1)\int_{0}^{\pi/2}\cos^{2k-2}x(1-\cos^2x)\,\,dx\\
	= (2k-1)\cancelto{I_{k-1}}{\left(\int_{0}^{\pi/2}\cos^{2k-2}x\,\,dx\right)} - (2k-1)\cancelto{I_k}{\int_{0}^{\pi/2}\cos^2x\,\,dx}\\
	\therefore I_k + (2k-1)I_k = (2k-1)I_{k-1}\\
	I_k = \frac{2k-1}{2k}I_{k-1}
\end{split}
\end{equation*}
Note that $I_0 = \frac{\pi}{2}$
\begin{equation*}
\begin{split}
	\therefore I_k = \frac{\pi}{2}\left(\frac{1}{2}\times\frac{3}{4}\times\dots\times\frac{2k-1}{2k}\right)\\
	= \int_{0}^{\pi/2}\cos^{2k}(x)\,\,dx = \frac{\pi}{2}\prod_{n=1}^{k}\frac{2n-1}{2n}
\end{split}
\end{equation*}


Now we solve $I_k$.
\begin{equation*}
\begin{split}
	I_k = \int_{0}^{\pi/2}\sin^{2k-1}x\sin(x)\,dx\\
	\text{Using IBP:}\\
	= \cancelto{0}{-\sin^{2k-1}x\cos(x)\Big|_0^{\pi/2}} + (2k-1)\int_0^{\pi/2}\sin^{2k-2}x\cos^2x\,dx\\
	= (2k-1)\int_0^{\pi/2}\left(\sin^{2k-2}x - \sin^{2k}x\right)\,dx\\
	= (2k-1)\cancelto{I_{k-1}}{\int_0^{\pi/2}\sin^{2k-2}x\,dx} - (2k-1)\cancelto{I_k}{\int_0^{\pi/2}\sin^{2k}\,dx}\\
	\therefore I_k + (2k-1)I_k = (2k-1)I_{k-1}\\
	I_k = \frac{2k-1}{2k}I_{k-1}
\end{split}
\end{equation*}
Note that $I_0=\frac{\pi}{2}$
\[\therefore I_k = \frac{2k-1}{2k}\times\frac{2k-3}{2k-2}\times\dots\times\frac{1}{2}I_0 = \frac{\pi}{2}\prod_{n=1}^k\frac{2n-1}{2n}\]