\documentclass{article}
\usepackage{amsmath, amssymb, amsthm}
\usepackage{hyperref}

\title{On the Cauchy-Schwarz Inequality}
\author{dnzc}
\date{}

\begin{document}
\maketitle

Consider a box of water with a width, height, and depth. Let the depth be $z$.\\
We separate the box into compartments by placing separators. Let the widths between them be $x_1, x_2, \dots, x_n$ for some arbitrary n. Then we fill up each compartment to a certain height $y_k$, so each compartment has a depth z, width $x_k$ and height of water $y_k$. See \href{https://drive.google.com/file/d/1gqm9ws1wQ1Q33ZyWLfZV_EY0Je3kAVvN/view?usp=sharing}{here} for a rough diagram.\\\\

The separators are instantaneously removed, and the water settles. We consider what happens to the total GPE of the water.
\[ GPE_{final} \geq GPE_{inital}\]
This is obvious, and I claim that it is nothing but the Cauchy-Schwarz inequality.

\section{Proof}

\subsection{Initial GPE}
\[GPE_{inital} = \sum GPE_k\]
Assume the density of the water and gravitational field strength are both 1, then:
\[GPE_k = mgh_{COM} = v_k \times \frac{y_k}{2} \text{ where } v_k \text{ is the volume of water in compartment k}\]
\[ = \frac{zx_ky_k^2}{2}\]
\[\therefore GPE_{inital} = \frac{z}{2} \sum x_ky_k^2\]

\subsection{Final GPE}
The water will all be at the same height after it settles, call this $y_{avg}$.
\[GPE_{final} = mgh_{COM} = v_t \frac{y_{avg}}{2} \text{ where } v_t \text{ is the total volume of all the water}\]
The volume of water does not change:
\[v_t = y_{avg} \times z \times \sum x_k= \sum x_ky_kz\]
\[\implies y_{avg} = \frac{\sum x_ky_k}{\sum x_k}\]
\[\therefore GPE_{final} = v_t \frac{y_{avg}}{2} = \frac{y_{avg}^2 \times z \times \sum x_k}{2} = \frac{z(\sum x_ky_k)^2}{2\sum x_k}\]

\subsection{Completing the proof}
\[ GPE_{final} \geq GPE_{inital}\]
Using our results from 1.1 and 1.2:
\[\frac{z(\sum x_ky_k)^2}{2\sum x_k} \geq \frac{z}{2} \sum x_ky_k^2\]
\[\frac{(\sum x_ky_k)^2}{\sum x_k} \geq \sum x_ky_k^2\]
\[(\sum x_ky_k)^2 \geq (\sum x_ky_k^2) (\sum x_k)\]
Let $x_ky_k^2 = a_k^2$ and $x_k = b_k^2$. Note that $\implies a_k^2b_k^2 = x_k^2y_k^2 \implies a_kb_k = x_ky_k$
Substitute this into the result above:
\[(\sum a_kb_k)^2 \geq (\sum a_k^2) (\sum b_k^2)\]
Which is exactly Cauchy-Schwarz.

\end{document}
